LambdaCalculus/ExplicitSubstitution.v
@@ -1,0 +1,155 @@
+From Coq Require Import Relations.
+From Coq Require Import Arith.
+From Coq Require Import Program.Basics.
+From KBase Require Import Tactics.
+From KBase Require Import Relations.
+From KBase Require LambdaCalculus.Terms.
+
+Import LambdaCalculus.Terms(tm(..)).
+
+(* Redo terms but with recursion schemes (or what is possible in Coq) *)
+
+(* mapping free variables *)
+Fixpoint map_freevar_k (f : nat -> nat) (t : tm) (k : nat) : tm :=
+  match t with
+  | Idx i => if lt_dec i k then Idx i else Idx (f (i - k) + k)
+  | Abs t => Abs (map_freevar_k f t (k + 1))
+  | App t1 t2 => App (map_freevar_k f t1 k) (map_freevar_k f t2 k)
+  end.
+
+Definition map_freevar (f : nat -> nat) (t : tm) : tm := map_freevar_k f t 0.
+#[export] Hint Unfold map_freevar : KBaseHints.
+
+(* map_freevar_k really is a functorial map for free variables *)
+
+Theorem map_freevar_k_id : forall t k, map_freevar_k (fun x => x) t k = t.
+Proof.
+  unfold map_freevar_k; 
+  induction t; crush; repeat (autodestruct; crush).
+Qed.
+#[export] Hint Resolve map_freevar_k_id : KBaseHints.
+
+Theorem map_freevar_k_compose : forall f1 f2 t k, 
+  map_freevar_k f2 (map_freevar_k f1 t k) k = map_freevar_k (compose f2 f1) t k.
+Proof.
+  unfold map_freevar_k; 
+  induction t; crush; repeat (autodestruct; crush);
+  match goal with
+  | |- context[?e + ?k - ?k] => 
+    let H := fresh "H"
+    in assert (H : e + k - k = e) by crush; rewrite H; crush
+  end.
+Qed.
+#[export] Hint Resolve map_freevar_k_compose : KBaseHints.
+
+(* In general, with different k we cannot simply compose but we 
+   can still extract t *)
+Theorem map_freevar_k_compose : forall f1 f2 t k1 k2, 
+  map_freevar_k f2 (map_freevar_k f1 t k1) k2 = 
+  map_freevar_k (compf f1 k1 f2) t min(k1, k2).
+Proof.
+  unfold map_freevar_k; 
+  induction t; crush; repeat (autodestruct; crush);
+  match goal with
+  | |- context[?e + ?k - ?k] => 
+    let H := fresh "H"
+    in assert (H : e + k - k = e) by crush; rewrite H; crush
+  end.
+Qed.
+#[export] Hint Resolve map_freevar_k_compose : KBaseHints.
+
+(* map_freevar always compose as a piece wise linear function *)
+
+
+(* Working with higher order function without function extensionality 
+   is no fun, but we can do it *)
+Theorem map_freevar_ext : forall f1 f2 t k,
+  (forall x, f1 x = f2 x) ->
+  map_freevar_k f1 t k = map_freevar_k f2 t k.
+Proof.
+  induction t; crush.
+Qed.
+#[export] Hint Resolve map_freevar_ext : KBaseHints.
+
+(* Same theorem but for map_freevar *)
+Theorem map_freevar_id : forall t, map_freevar (fun x => x) t = t.
+Proof.
+  unfold map_freevar; crush.
+Qed.
+#[export] Hint Resolve map_freevar_id : KBaseHints.
+
+Theorem map_freevar_compose : forall f1 f2 t, 
+  map_freevar f2 (map_freevar f1 t) = map_freevar (compose f2 f1) t.
+Proof.
+  unfold map_freevar; crush.
+Qed.
+#[export] Hint Resolve map_freevar_compose : KBaseHints.
+
+(* Shift can be expressed as a map *)
+Definition shift (n : nat) (t : tm) : tm := map_freevar (fun x => x + n) t.
+#[export] Hint Unfold shift : KBaseHints.
+
+Theorem shift_0 : forall t, shift 0 t = t.
+Proof.
+  unfold shift; unfold map_freevar; intros;
+  assert (H : forall x : nat, (fun x => x + 0) x = (fun x => x) x) by crush.
+  pose proof (map_freevar_ext _ _ t 0 H);
+  crush.
+Qed.
+
+Theorem shift_shift : forall t n1 n2, shift n2 (shift n1 t) = shift (n1 + n2) t.
+Proof.
+  unfold shift; intros. rewrite map_freevar_compose.
+  assert (H : forall x : nat, 
+    (compose (fun x : nat => x + n2) (fun x : nat => x + n1)) x = 
+    (fun x => x + (n1 + n2)) x).
+    - intros; unfold compose; crush.
+    - pose proof (map_freevar_ext _ _ t 0 H); crush.
+Qed.
+
+(* We can also define a recursion scheme for substitution *)
+Fixpoint subst_freevar_k (f : nat -> tm) (t : tm) (k : nat) : tm :=
+  match t with
+  | Idx i => if lt_dec i k then Idx i else (shift k (f (i - k)))
+  | Abs t => Abs (subst_freevar_k f t (k + 1))
+  | App t1 t2 => App (subst_freevar_k f t1 k) (subst_freevar_k f t2 k)
+  end.
+
+(* map_freevar_k is not quite a functorial map for free variables,
+   but close *)
+Theorem subst_freevar_k_id : forall t k, subst_freevar_k (fun x => Idx x) t k = t.
+Proof.
+  unfold subst_freevar_k; unfold shift; unfold map_freevar;
+  induction t; crush; repeat (autodestruct; crush).
+Qed.
+#[export] Hint Resolve subst_freevar_k_id : KBaseHints.
+
+Theorem subst_shift : forall f t n k,
+  subst_freevar_k f (map_freevar_k (fun x : nat => x + k) t n) (k + n) =
+  map_freevar_k (fun x : nat => x + k) (subst_freevar_k f t n) n.
+Proof.
+  induction t; intros k.
+  - unfold shift; unfold map_freevar; crush; repeat (autodestruct; crush). 
+    assert (H1 : n - k + k0 + k - (k0 + k) = n - k) by crush.
+    rewrite H1.
+    unfold shift. unfold map_freevar.
+    pose proof (map_freevar_k_compose (fun x : nat => x + k)  (fun x : nat => x + k0)
+      (f (n - k)) k).
+    assert (H2 : n - 0 = n) by crush.
+    
+    crush.
+  - simpl.
+
+(* We cannot compose, but we can extract the t and k arguments,
+   thus grouping the substitution functions together *)
+Theorem subst_freevar_k_compose : forall f1 f2 t k, 
+  subst_freevar_k f2 (subst_freevar_k f1 t k) k = 
+  subst_freevar_k (fun i => subst_freevar_k f2 (f1 i) 0) t k.
+Proof.
+  induction t; crush; repeat (autodestruct; crush).
+  match goal with
+  | |- context[?e + ?k - ?k] => 
+    let H := fresh "H"
+    in assert (H : e + k - k = e) by crush; rewrite H; crush
+  end.
+Qed.
